* Original grammar :noexport:
expr	::=	num 
                | lvalue 
                | incrop expr 
                | expr incrop 
                | expr binop expr 
                | (expr)
lvalue	::=	$expr
incrop	::=	++ 
                | --
binop	::=	+ 
                | -
                | \epsilon  
num	::=	0 | 1 | 2 | 3 | 4 | 5 | 6 | 7 | 8 | 9

* LL(1) grammar
R1 : string  ::=     expr string'
R2 : string' ::=     _ expr string' 
R3 :                 | \epsilon
R4 : expr    ::=     pre expr'
R5 : expr'   ::=     binop pre expr'
R6 :                 | \epsilon
R7 : pre     ::=     incrop pre
R8 :                 | post
R9 : post    ::=     ref post'
R10 : post'   ::=     incrop post'
R11:                 | \epsilon
R12: ref     ::=     F ref
R13:                 | term
R14: term    ::=     num
R15:                 | (expr)
R16: binop   ::=     + | -
R17: incrop  ::=     ++ | --
R18: num     ::=     0 | 1 | 2 | 3 | 4 | 5 | 6 | 7 | 8 | 9
* First
  FIRST(string)   = FIRST(expr) = {(, ++, --, F, 0, 1, 2, 3, 4, 5, 6, 7, 8, 9}
  FIRST(string')  = {\epsilon, _}
  FIRST(expr)     = FIRST(pre) = {++, --, F, (, 0, 1, 2, 3, 4, 5, 6, 7, 8, 9}
  FIRST(expr')    = FIRST(binop) U {\epsilon} = {\epsilon, +, -}
  FIRST(pre)      = FIRST(incrop) U FIRST(post) = {++, --, F, (, 0, 1, 2, 3, 4, 5, 6, 7, 8, 9}
  FIRST(post)     = FIRST(ref) = {F, (, 0, 1, 2, 3, 4, 5, 6, 7, 8, 9}
  FIRST(post')    = FIRST(incrop) U {\epsilon}= {\epsilon, ++, --}
  FIRST(ref )     = {F} U FIRST(term) = {F, (, 0, 1, 2, 3, 4, 5, 6, 7, 8, 9}
  FIRST(term)     = FIRST(num) U {(} = {(, 0, 1, 2, 3, 4, 5, 6, 7, 8, 9}
  FIRST(num)      = {0, 1, 2, 3, 4, 5, 6, 7, 8, 9}
  FIRST(binop)    = {+, -}
  FIRST(incrop)   = {++, --}
* Follow
  FOLLOW(string)  = {$}
  FOLLOW(string') = FOLLOW(string) = {$}
  FOLLOW(expr)    = FIRST(string') U {)} = {$, _, )}
  FOLLOW(expr')   = FOLLOW(expr)= {$, _, )}
  FOLLOW(pre)     = FIRST(expr') = {\epsilon, +, -}
  FOLLOW(post)    = FOLLOW(pre) = {\epsilon, +, -}
  FOLLOW(post')   = FOLLOW(post) = {\epsilon, +, -}
  FOLLOW(ref)     = FIRST(post') = {\epsilon, ++, --}
  FOLLOW(term)    = FOLLOW(ref) = {\epsilon, ++, --}
* Parse table
  |         | num | binop | incrop | F   | $  | _  | (   | )  |
  |---------+-----+-------+--------+-----+----+----+-----+----|
  | string  | R1  |       | R1     | R1  | R1 | R1 | R1  |    |
  | string' |     |       |        |     | R3 | R2 |     |    |
  | expr    | R4  |       | R4     | R4  |    |    | R4  |    |
  | expr'   |     | R5    |        |     | R6 |    |     | R5 |
  | pre     | R8  |       | R7     | R8  |    |    | R8  |    |
  | post    | R9  |       | R9     | R9  |    |    | R9  |    |
  | post'   |     | R10   | R10    |     |    |    |     |    |
  | ref     | R13 |       | R13    | R12 |    |    | R13 |    |
  | term    | R14 |       |        |     |    |    | R15 |    |

